Made the proof of Russell's paradox nice and clean

examples/paradoxes/russell.fst
@@ -6,51 +6,39 @@ module Russell
 open FStar.Constructive
 
 (* Russell's paradox; didn't expect this to work, but it does ... even if
-   - we don't have Type : Type; for us Type : *
-   - we don't have good ways to define some of the ingredients
-     (e.g. elimination at the type level for in_set)
-     + working around it *)
+   - we don't have Type : Type -- or so I thought *)
 
-(* The proof follows: The Essence of Coq as a Formal System, Bart Jacobs
-   (http://people.cs.kuleuven.be/~bart.jacobs/coq-essence.pdf)
+(* The proof follows the one from The Essence of Coq as a Formal System
+   by Bart Jacobs (http://people.cs.kuleuven.be/~bart.jacobs/coq-essence.pdf)
    which in turn is based on a proof by Paolo Capriotti. *)
 
 type U = | Set : i:Type  -> p:(i -> Type) -> f:(i -> Tot U) -> U
 
-(* in_set was supposed to have kind U -> U -> Type, but I couldn't
-   break up the second argument (no type-level elimination) *)
-type in_set (x:U) (i:Type) (p:(i->Type)) (f:(i->Tot U)) =
-  cexists #i (fun (ii:i) -> cand (p ii) (ceq #U (f ii) x))
+type in_set (x:U) (y:U) =
+  cexists #(Set.i y) (fun (ii:Set.i y) -> cand (Set.p y ii) (ceq #U (Set.f y ii) x))
 
 val id : U -> Tot U
 let id x = x
 
+(* The definition of spec fails in Coq because of a universe inconsistency *)
 val spec : (U -> Type) -> Tot U
 let spec (p:(U->Type)) = Set U p id
 
-val spec_intro : p:(U->Type) -> x:U -> h:(p x) -> Tot (in_set x (Set.i (spec p))
-                                                                (Set.p (spec p))
-                                                                (Set.f (spec p)))
+val spec_intro : p:(U->Type) -> x:U -> h:(p x) -> Tot (in_set x (spec p))
 let spec_intro (p:U->Type) (x:U) (h:(p x)) = ExIntro x (Conj h (Refl (id x)))
 
-val spec_elim : p:(U->Type) -> x:U -> h:(in_set x (Set.i (spec p))
-                                                  (Set.p (spec p))
-                                                  (Set.f (spec p))) -> Tot (p x)
+val spec_elim : p:(U->Type) -> x:U -> h:(in_set x (spec p)) -> Tot (p x)
 let spec_elim (p:U->Type) (x:U) h =
   let ExIntro i (Conj h1 h2) = h in h1
 
-type pr (x:U) = cnot (in_set x (Set.i x)
-                               (Set.p x)
-                               (Set.f x))
+type pr (x:U) = cnot (in_set x x)
 
-val contradiction : p:Type -> h1:(cnot p -> Tot p)   ->
-                              h2:(p -> Tot (cnot p)) -> Tot cfalse
+val contradiction : p:Type -> h1:(cnot p -> Tot       p ) ->
+                              h2:(     p -> Tot (cnot p)) -> Tot cfalse
 let contradiction (p:Type) h1 h2 =
   (fun (h3:(cnot p)) -> h3 (h1 h3)) (fun (hp:p) -> h2 hp hp)
 
 val absurd : unit -> Tot cfalse
-let absurd () = contradiction (in_set (spec pr) (Set.i (spec pr))
-                                                (Set.p (spec pr))
-                                                (Set.f (spec pr)))
+let absurd () = contradiction (in_set (spec pr) (spec pr))
                               (spec_intro pr (spec pr))
                               (spec_elim  pr (spec pr))
